theories/typing/mod_ty.v
@@ -10,9 +10,8 @@ Section mod_ty.
     (l ↦∗{q}: λ vl, ∃vπ, ⌜vπ' = f ∘ vπ⌝ ∗ ty.(ty_own) (vπ,d) tid vl)%I ⊣⊢
     ∃vπ, ⌜vπ' = f ∘ vπ⌝ ∗ l ↦∗{q}: ty.(ty_own) (vπ,d) tid.
   Proof. iSplit.
-    - iDestruct 1 as (vl) "[Mt Own]". iDestruct "Own" as (vπ->) "Own".
-      iExists vπ. iSplit; [done|]. iExists vl. iFrame.
-    - iDestruct 1 as (vπ->vl) "[Mt Own]". iExists vl. iFrame "Mt". iExists vπ.
+    - iIntros "[%vl[?[%vπ[->Own]]]]". iExists vπ. iSplit; [done|]. iExists vl. iFrame.
+    - iIntros "[%vπ[->[%vl[Mt Own]]]]". iExists vl. iFrame "Mt". iExists vπ.
       by iSplit; [done|].
   Qed.
 
@@ -21,28 +20,28 @@ Section mod_ty.
     ty_own vπd tid vl := ∃vπ, ⌜vπd.1 = f ∘ vπ⌝ ∗ ty.(ty_own) (vπ,vπd.2) tid vl;
     ty_shr vπd κ tid l := ∃vπ, ⌜vπd.1 = f ∘ vπ⌝ ∗ ty.(ty_shr) (vπ,vπd.2) κ tid l;
   |}%I.
-  Next Obligation. move=> *. iDestruct 1 as (??) "?". by iApply ty_size_eq. Qed.
+  Next Obligation. move=> *. iIntros "[%[%?]]". by iApply ty_size_eq. Qed.
   Next Obligation.
-    move=> */=. iDestruct 1 as (vπ->) "?". iExists vπ. iSplit; [done|].
+    move=> */=. iIntros "[%vπ[->?]]". iExists vπ. iSplit; [done|].
     by iApply ty_own_depth_mono.
   Qed.
   Next Obligation.
-    move=> */=. iDestruct 1 as (vπ->) "?". iExists vπ. iSplit; [done|].
+    move=> */=. iIntros "[%vπ[->?]]". iExists vπ. iSplit; [done|].
     by iApply ty_shr_depth_mono.
   Qed.
   Next Obligation.
-    move=> */=. iIntros "#?". iDestruct 1 as (vπ->) "?". iExists vπ. iSplit; [done|].
+    move=> */=. iIntros "#? [%vπ[->?]]". iExists vπ. iSplit; [done|].
     by iApply ty_shr_lft_mono.
   Qed.
   Next Obligation.
     move=> */=. iIntros "#LFT In Bor Tok". rewrite mod_ty_mt.
     iMod (bor_exists_tok with "LFT Bor Tok") as (vπ) "[Bor Tok]"; [done|].
-    iMod (bor_sep_persistent with "LFT Bor Tok") as "[>->[Bor Tok]]"; [done|].
+    iMod (bor_sep_persistent with "LFT Bor Tok") as "(>-> & Bor & Tok)"; [done|].
     iMod (ty_share with "LFT In Bor Tok") as "Upd"; [done|].
     iApply (step_fupdN_wand with "Upd"). iIntros "!> >[Shr $] !>". iExists vπ. by iSplit.
   Qed.
   Next Obligation.
-    move=> */=. iIntros "#LFT In". iDestruct 1 as (vπ->) "Own". iIntros "Tok".
+    move=> */=. iIntros "#LFT In [%vπ[->Own]] Tok".
     iMod (ty_own_proph with "LFT In Own Tok") as "Upd"; [done|]. iModIntro.
     iApply (step_fupdN_wand with "Upd"). iMod 1 as (ξs q ?) "[PTok Close]".
     iModIntro. iExists ξs, q. iSplit; [iPureIntro; by apply (proph_dep_constr _)|].
@@ -50,7 +49,7 @@ Section mod_ty.
     iModIntro. iExists vπ. by iSplit.
   Qed.
   Next Obligation.
-    move=> */=. iIntros "#LFT In In'". iDestruct 1 as (vπ->) "Shr". iIntros "Tok".
+    move=> */=. iIntros "#LFT In In' [%vπ[->Shr]] Tok".
     iMod (ty_shr_proph with "LFT In In' Shr Tok") as "Upd"; [done|]. iIntros "!>!>".
     iApply (step_fupdN_wand with "Upd"). iMod 1 as (ξs q ?) "[PTok Close]".
     iModIntro. iExists ξs, q. iSplit; [iPureIntro; by apply (proph_dep_constr _)|].
@@ -78,9 +77,8 @@ Section typing.
 
   Global Instance mod_ty_copy {A B} (f: A → B) ty : Copy ty → Copy (<{f}> ty).
   Proof.
-    move=> [? ShrAcc]. split; [by apply _|]. move=> */=. iIntros "LFT".
-    iDestruct 1 as (vπ ->) "Shr". iIntros "Na Tok".
-    iMod (ShrAcc with "LFT Shr Na Tok") as (q vl) "[$[Mt[? Close]]]"; [done|done|].
+    move=> [? ShrAcc]. split; [by apply _|]=> */=. iIntros "LFT [%vπ[->Shr]] Na Tok".
+    iMod (ShrAcc with "LFT Shr Na Tok") as (q vl) "($& Mt &?& Close)"; [done|done|].
     iModIntro. iExists q, vl. iFrame "Mt Close". iNext. iExists vπ. by iSplit.
   Qed.
 
@@ -93,14 +91,26 @@ Section typing.
   Lemma mod_ty_own {A B} g f `{@Iso A B f g} ty vπ d tid vl :
     (<{f}> ty).(ty_own) (vπ, d) tid vl ⊣⊢ ty.(ty_own) (g ∘ vπ, d) tid vl.
   Proof. iSplit=>/=.
-    - iDestruct 1 as (?->) "?". by rewrite compose_assoc semi_iso.
+    - iIntros "[%[->?]]". by rewrite compose_assoc semi_iso.
     - iIntros "?". iExists (g ∘ vπ). iFrame. by rewrite compose_assoc semi_iso.
   Qed.
   Lemma mod_ty_shr {A B} g f `{@Iso A B f g} ty vπ d κ tid l :
     (<{f}> ty).(ty_shr) (vπ, d) κ tid l ⊣⊢ ty.(ty_shr) (g ∘ vπ, d) κ tid l.
   Proof. iSplit=>/=.
-    - iDestruct 1 as (?->) "?". by rewrite compose_assoc semi_iso.
+    - iIntros "[%[->?]]". by rewrite compose_assoc semi_iso.
     - iIntros "?". iExists (g ∘ vπ). iFrame. by rewrite compose_assoc semi_iso.
+  Qed.
+
+  Lemma mod_ty_id {A} (ty: _ A) : <{id}>%T ty ≡ ty.
+  Proof. split; move=>// [??]*; by [rewrite mod_ty_own|rewrite mod_ty_shr]. Qed.
+
+  Lemma mod_ty_compose {A B C} (f: A → B) (g: _ → C) ty :
+    (<{g}> (<{f}> ty) ≡ <{g ∘ f}> ty)%T.
+  Proof.
+    split=>// *; (iSplit=>/=; [
+      iIntros "[%_[->[%vπ[->?]]]]"; iExists vπ; by iFrame|
+      iIntros "[%vπ[->?]]"; iExists (f ∘ vπ); (iSplit; [done|]); iExists vπ; by iFrame
+    ]).
   Qed.
 
   Lemma mod_ty_in {A B} E L (f: A → B) ty : subtype E L f ty (<{f}> ty).
@@ -113,7 +123,7 @@ Section typing.
     subtype E L g (<{f}> ty) ty.
   Proof.
     iIntros "*_!>_". iSplit; [done|]. iSplit; [by iApply lft_incl_refl|].
-    iSplit; iIntros "!>*/="; iDestruct 1 as (?->) "?"; by rewrite compose_assoc semi_iso.
+    iSplit; iIntros "!>*/=[%[->?]]"; by rewrite compose_assoc semi_iso.
   Qed.
 
   Lemma mod_ty_inout {A B} E L f g `{@SemiIso A B f g} ty :
